% \documentclass[12pt,a4paper]{report}
\documentclass[a4paper,12pt,fleqn]{article}
\usepackage{amsmath}
\setlength{\mathindent}{0cm}
\begin{document}

Problem 2.11 (page 63).

$E$ is the shift operator.

\begin{align}
  & \hskip 4pt \sum \Delta a_k b_k\\
= & \sum_{0\leq k < n} (a_{k+1} - a_k)b_k \\
= & \sum_{0\leq k < n} a_{k+1} b_k - a_k b_k \\
= & \sum_{0\leq k < n} a_{k+1} b_k - \sum_{0\leq k < n} a_k b_k \\
= & \sum_{0\leq k < n} a_{k+1} b_k - \sum_{0\leq k+1 < n} a_{k+1} b_{k+1} \\
= & \sum_{0\leq k < n} a_{k+1} b_k - \sum_{-1\leq k < n-1} a_{k+1} b_{k+1} \\
= & \sum_{0\leq k < n} a_{k+1} b_k - \sum_{0\leq k < n} a_{k+1} b_{k+1} + (a_n b_n - a_0 b_0) \\
= & - \sum_{0\leq k < n} a_{k+1} (b_{k+1} - b_k) + (a_n b_n - a_0 b_0) \\
= & - \sum_{0\leq k < n} a_{k+1} \Delta b_{k} + \left.(a_k b_k)\right|_0^n  \\
= & \left.(a_k b_k)\right|_0^n - \sum_{0\leq k < n} E a_k \Delta b_{k} \\
\end{align}
%
Step (5) will shift $k \to k+1$. \\
Step (6) will re-adjust the bounds. \\
Step (7) splits off the first term, adds an addition term, and then subtracts that additional term. \\
Step (9) rewrites the outer difference as an evaluation, also rewrites the sum using the difference operator. \\
Step (10) uses rewrites the expression using the shift operator.\\
\\
\textbf{Note:} the evaluation in (10) has its upper bound 1 greater than the initial upper-bound of the original sum in (1).

\end{document}