% \documentclass[12pt,a4paper]{report}
\documentclass[a4paper,10pt,fleqn]{article}
\usepackage{amsmath}
\usepackage[colorlinks=true,citecolor=blue,linkcolor=blue]{hyperref}

\setlength{\mathindent}{0cm}
\begin{document}
\newcommand{\ffac}[1]{%
  x^{\underline{#1}}%
}
\newcommand{\ffact}[2]{% 
  {#1}^{\underline{#2}}%
}
\noindent Compute:
{\setlength{\mathindent}{0cm}
\begin{equation*}
\sum_{0\leq k <n} \frac{H_k}{(k+1)(k+2)} = \sum_{0\leq k <n} H_k \cdot \ffac{-2} 
\end{equation*}
}
\noindent Facts used (for $m>0$):
\begin{align*}
& \ffact{0}{-m} =\frac{1}{(0+1)(0+2)\cdots(0+m)} = \frac{1}{m!} \\
& E \ffac{-m} = E \frac{1}{(x+1)\cdots(x+m)} = \frac{1}{(x+2)\cdots (x+m+1)} = \ffac{-m-1} (x+1)\\
\end{align*}

Computing the indefinite sum:

\begin{align*}
S = & \sum H_x \cdot x^{\underline{m}} \\
= & \sum H_x \Delta \left( \frac{ \ffac{-m+1} }{-m+1} \right) \\
= & \left(H_x \frac{ \ffac{-m+1} }{-m+1}\right) - \frac{1}{-m+1} \sum E \ffac{-m+1} \Delta H_x \\
= & \left(H_x \frac{ \ffac{-m+1} }{-m+1}\right) - \frac{1}{-m+1} \sum \ffac{-m} (x+1) \Delta H_x \\
= & \left(H_x \frac{ \ffac{-m+1} }{-m+1}\right) - \frac{1}{-m+1} \sum \ffac{-m} (x+1) \frac{1}{x+1} \\
= & \left(H_x \frac{ \ffac{-m+1} }{-m+1}\right) - \frac{1}{-m+1} \sum \ffac{-m} \\
= & \left(H_x \frac{ \ffac{-m+1} }{-m+1}\right) - \frac{ \ffac{-m+1} }{(-m+1)^2} \\
= & \frac{\ffac{-m+1}}{-m+1} \left( H_x - \frac{1}{-m+1} \right) \\
\end{align*}

Computing the definite sum:

\begin{align*}
\left.S\right|_0^n = & \frac{\ffact{n}{-m+1}}{-m+1} \left( H_n - \frac{1}{-m+1} \right) - \frac{\ffact{0}{-m+1}}{-m+1} \left( H_0 - \frac{1}{-m+1} \right) \\
 = & \frac{\ffact{n}{-m+1}}{-m+1} \left( H_n - \frac{1}{-m+1} \right) + \frac{(m-1)!}{(-m+1)^2} \\
\end{align*}

If we set $m=2$ we get $ S = 1 - \frac{1}{n+1} \left( H_n + 1 \right) $

\end{document}
