% \documentclass[12pt,a4paper]{report}
\documentclass[a4paper,12pt,fleqn]{article}
\usepackage{amsmath}
\setlength{\mathindent}{0cm}
\begin{document}

\begin{align*}
& u(k) = 2k+1 \implies \Delta u(k) = (2k+3) - (2k+1) = 2 \\
& \Delta v(k) = \frac{1}{k(k+1)} = (k-1)^{\underline{-2}} \\
& \sum \Delta v(k) = \sum (k-1)^{\underline{-2}} = \frac{(k-1)^{\underline{-2+1}}}{-2+1} = \frac{(k- 1)^{\underline{-1}}}{-1} = -\frac{1}{k} = v(k) \\ 
\hline \\
& \sum_{k=1}^n u(k) \Delta v(k) = \left.(u(k)v(k))\right|_1^n - \sum_{k=1}^n E v(k)\Delta u(k) \\
& \sum_{k=1}^n u(k) \Delta v(k) = \left.\left(-\frac{2k+1}{k}\right)\right|_1^{n+1} - \sum_{k=1}^n 2 \cdot \left(-\frac{1}{k+1}\right) = \\
& \left.\left(2 + \frac{1}{k} \right)\right|_{n+1}^{1} - 2 + 2 \sum_{k=2}^{n+1} \frac{1}{k} = \\
& \frac{1}{n+1} - 1 + 2H_n \\
\end{align*}

\end{document}